Add Memory.v

src/model/Cell.v
@@ -1,6 +1,4 @@
 Require Import RelationClasses.
-Require Import Decidable.
-Require Import Coq.Lists.ListDec.
 
 From sflib Require Import sflib.
 
@@ -22,10 +20,12 @@ Module Message.
 
   Definition elt: t := mk Const.undef None.
 
-  Definition wf (msg: t): Prop :=
-    match msg with
-    | mk val released => View.opt_wf released
-    end.
+  Variant wf: t -> Prop :=
+  | wf_intro
+      val released
+      (RELEASED: View.opt_wf released):
+    wf (mk val released)
+  .
 
   Definition elt_wf: wf elt.
   Proof. ss. Qed.
@@ -36,7 +36,7 @@ Module Message.
     | _ => false
     end.
 End Message.
-#[export] Hint Unfold Message.wf: core.
+#[export] Hint Constructors Message.wf: core.
 
 
 Module Cell.
@@ -157,43 +157,6 @@ Module Cell.
         + inv GET2. inv ADD. symmetry. hexploit DISJOINT0; eauto.
         + eapply DISJOINT; eauto.
     Qed.
-
-    Variant remove (cell1:t) (from to:Time.t) (msg:Message.t) (cell2:t): Prop :=
-    | remove_intro
-        (GET: DOMap.find to cell1 = Some (from, msg))
-        (CELL2: cell2 = DOMap.remove to cell1)
-    .
-    #[global] Hint Constructors remove: core.
-
-    Lemma remove_o
-          cell2 cell1 from to msg
-          t
-          (REMOVE: remove cell1 from to msg cell2):
-      DOMap.find t cell2 =
-      if Time.eq_dec t to
-      then None
-      else DOMap.find t cell1.
-    Proof.
-      inv REMOVE. rewrite DOMap.grspec.
-      repeat condtac; auto; congr.
-    Qed.
-
-    Lemma remove_wf
-          cell1 from to msg cell2
-          (REMOVE: remove cell1 from to msg cell2)
-          (CELL1: wf cell1):
-      wf cell2.
-    Proof.
-      inv CELL1. econs; i.
-      - revert GET. erewrite remove_o; eauto. condtac; try congr.
-        i. eapply VOLUME; eauto.
-      - revert GET. erewrite remove_o; eauto. condtac; ss. apply WF.
-      - revert GET1 GET2.
-        erewrite (remove_o to1); eauto.
-        erewrite (remove_o to2); eauto.
-        repeat condtac; repeat subst; try congr; i.
-        eapply DISJOINT; eauto.
-    Qed.
   End Raw.
 
   Structure t := mk {
@@ -270,13 +233,13 @@ Module Cell.
              (from to:Time.t) (msg:Message.t)
              (LT: Time.lt from to)
              (WF: Message.wf msg): t :=
-    mk (Raw.singleton_wf msg LT WF).
+    mk (Raw.singleton_wf LT WF).
 
   Lemma singleton_get
         from to msg t
         (LT: Time.lt from to)
         (WF: Message.wf msg):
-    get t (singleton msg LT WF) =
+    get t (singleton LT WF) =
     if Time.eq_dec t to
     then Some (from, msg)
     else None.
@@ -302,9 +265,6 @@ Module Cell.
   Definition add (cell1:t) (from to:Time.t) (msg: Message.t) (cell2:t): Prop :=
     Raw.add cell1 from to msg cell2.
 
-  Definition remove (cell1:t) (from to:Time.t) (msg: Message.t) (cell2:t): Prop :=
-    Raw.remove cell1 from to msg cell2.
-
   Lemma add_o
         cell2 cell1 from to msg
         t
@@ -314,16 +274,6 @@ Module Cell.
     then Some (from, msg)
     else get t cell1.
   Proof. apply Raw.add_o. auto. Qed.
-
-  Lemma remove_o
-        cell2 cell1 from to msg
-        t
-        (REMOVE: remove cell1 from to msg cell2):
-    get t cell2 =
-    if Time.eq_dec t to
-    then None
-    else get t cell1.
-  Proof. eapply Raw.remove_o. eauto. Qed.
 
   Definition max_ts (cell:t): Time.t :=
     DOMap.max_key (raw cell).
@@ -371,17 +321,17 @@ Module Cell.
   Qed.
 
   Lemma add_exists_le
-        promises1 cell1 from to msg cell2
-        (LE: le promises1 cell1)
+        cell1' cell1 from to msg cell2
+        (LE: le cell1' cell1)
         (ADD: add cell1 from to msg cell2):
-    exists promises2, add promises1 from to msg promises2.
+    exists cell2', add cell1' from to msg cell2'.
   Proof.
     inv ADD. apply add_exists; auto. i.
     eapply DISJOINT. eauto.
   Qed.
 
 
-  (* Lemmas on add, remove *)
+  (* Lemmas on add *)
 
   Lemma add_get0
         cell1 from1 to1 msg1 cell2
@@ -397,16 +347,6 @@ Module Cell.
         destruct (Cell.WF cell1). exploit VOLUME; eauto. intros x. des; ss.
         inv x. inv TO.
     - rewrite CELL2, DOMap.gsspec. condtac; ss.
-  Qed.
-
-  Lemma remove_get0
-        cell1 from to msg cell2
-        (REMOVE: remove cell1 from to msg cell2):
-    <<GET: get to cell1 = Some (from, msg)>> /\
-    <<GET: get to cell2 = None>>.
-  Proof.
-    inv REMOVE. splits; auto.
-    unfold get. rewrite CELL2. rewrite DOMap.grspec. condtac; ss.
   Qed.
 
   Lemma add_get1
@@ -444,36 +384,6 @@ Module Cell.
       + eapply max_ts_spec. eauto.
       + inv ADD. auto.
     - eapply max_ts_spec. erewrite add_o; eauto. condtac; ss.
-  Qed.
-
-  Lemma remove_singleton
-        from to msg
-        (LT:Time.lt from to)
-        (WF: Message.wf msg):
-    remove (singleton msg LT WF) from to msg bot.
-  Proof.
-    assert (Raw.bot = DOMap.remove to ((raw (singleton msg LT WF)))).
-    { apply DOMap.eq_leibniz. ii.
-      unfold Raw.bot. rewrite DOMap.gempty.
-      rewrite DOMap.grspec. condtac; auto.
-      unfold singleton, Raw.singleton, raw.
-      rewrite DOMap.singleton_neq; auto.
-    }
-    unfold remove. s. rewrite H. econs; ss.
-    unfold Raw.singleton. rewrite DOMap.singleton_eq. auto.
-  Qed.
-
-  Lemma remove_exists
-        cell1 from to msg
-        (GET: get to cell1 = Some (from, msg)):
-    exists cell2, remove cell1 from to msg cell2.
-  Proof.
-    eexists (mk _). destruct cell1. ss.
-    Unshelve.
-    { eapply Raw.remove_wf.
-      - econs; eauto.
-      - apply WF.
-    }
   Qed.
 
   Lemma get_opt_wf
