src/model/Memory.v
@@ -1,0 +1,708 @@
+Require Import RelationClasses.
+
+From sflib Require Import sflib.
+
+From PromisingLib Require Import Axioms.
+From PromisingLib Require Import Basic.
+From PromisingLib Require Import DataStructure.
+From PromisingLib Require Import DenseOrder.
+From PromisingLib Require Import Loc.
+From PromisingLib Require Import Event.
+
+Require Import Time.
+Require Import View.
+Require Import Cell.
+
+Set Implicit Arguments.
+
+
+Module Memory.
+  Definition t := Loc.t -> Cell.t.
+
+  Definition get (loc:Loc.t) (ts:Time.t) (mem:t): option (Time.t * Message.t) :=
+    Cell.get ts (mem loc).
+
+  Lemma get_disjoint
+        l f1 f2 t1 t2 msg1 msg2 m
+        (GET1: get l t1 m = Some (f1, msg1))
+        (GET2: get l t2 m = Some (f2, msg2)):
+    (t1 = t2 /\ f1 = f2 /\ msg1 = msg2) \/
+    Interval.disjoint (f1, t1) (f2, t2).
+  Proof.
+    eapply Cell.get_disjoint; eauto.
+  Qed.
+
+  Lemma ext
+        lhs rhs
+        (EXT: forall loc ts, get loc ts lhs = get loc ts rhs):
+    lhs = rhs.
+  Proof.
+    apply LocFun.ext. i.
+    apply Cell.ext. i.
+    apply EXT.
+  Qed.
+
+  Lemma get_ts
+        loc to mem from msg
+        (GET: get loc to mem = Some (from, msg)):
+    (from = Time.bot /\ to = Time.bot) \/ Time.lt from to.
+  Proof.
+    unfold get in *.
+    apply Cell.get_ts in GET. auto.
+  Qed.
+
+  Definition le (lhs rhs:t): Prop :=
+    forall loc to from msg
+      (LHS: get loc to lhs = Some (from, msg)),
+      get loc to rhs = Some (from, msg).
+
+  Global Program Instance le_PreOrder: PreOrder le.
+  Next Obligation. ii. auto. Qed.
+  Next Obligation. ii. eapply H0; eauto. Qed.
+
+  Variant disjoint (lhs rhs:t): Prop :=
+  | disjoint_intro
+      (DISJOINT: forall loc to1 to2 from1 from2 msg1 msg2
+                   (GET1: get loc to1 lhs = Some (from1, msg1))
+                   (GET2: get loc to2 rhs = Some (from2, msg2)),
+          Interval.disjoint (from1, to1) (from2, to2) /\
+          (to1, to2) <> (Time.bot, Time.bot))
+  .
+  #[global] Hint Constructors disjoint: core.
+
+  Global Program Instance disjoint_Symmetric: Symmetric disjoint.
+  Next Obligation.
+    inv H. econs. i. exploit DISJOINT; eauto. i. des. splits.
+    - symmetry. auto.
+    - ii. inv H. congr.
+  Qed.
+
+  Lemma disjoint_get
+        lhs rhs
+        loc froml fromr to msgl msgr
+        (DISJOINT: disjoint lhs rhs)
+        (LMSG: get loc to lhs = Some (froml, msgl))
+        (RMSG: get loc to rhs = Some (fromr, msgr)):
+    False.
+  Proof.
+    inv DISJOINT. exploit DISJOINT0; eauto. intros x. des.
+    destruct (Time.eq_dec to Time.bot).
+    - subst. congr.
+    - eapply x.
+      + apply Interval.mem_ub. destruct (Cell.WF (lhs loc)).
+        exploit VOLUME; eauto. intros x1. des; auto. inv x1. congr.
+      + apply Interval.mem_ub. destruct (Cell.WF (rhs loc)).
+        exploit VOLUME; eauto. intros x1. des; auto. inv x1. congr.
+  Qed.
+
+  Lemma disjoint_get_general
+        lhs rhs
+        loc ts0 ts1 ts2 ts3 msgl msgr
+        (TS12: Time.lt ts1 ts2)
+        (TS23: Time.le ts2 ts3)
+        (DISJOINT: disjoint lhs rhs)
+        (LMSG: get loc ts2 lhs = Some (ts0, msgl))
+        (RMSG: get loc ts3 rhs = Some (ts1, msgr)):
+    False.
+  Proof.
+    inv DISJOINT. exploit DISJOINT0; eauto. intros x. des.
+    destruct (Time.le_lt_dec ts2 ts0).
+    - destruct (Cell.WF (lhs loc)). exploit VOLUME; eauto. intros x1. des.
+      + inv x1. inv TS12.
+      + eapply Time.lt_strorder. eapply TimeFacts.le_lt_lt; eauto.
+    - eapply x.
+      + eapply Interval.mem_ub. auto.
+      + econs; auto.
+  Qed.
+
+  Definition bot: t := fun _ => Cell.bot.
+
+  Lemma bot_get loc ts: get loc ts bot = None.
+  Proof. unfold get. apply Cell.bot_get. Qed.
+
+  Lemma bot_le mem: le bot mem.
+  Proof. ii. rewrite bot_get in LHS. congr. Qed.
+
+  Lemma bot_disjoint mem: disjoint bot mem.
+  Proof.
+    econs. i. rewrite bot_get in *. inv GET1.
+  Qed.
+
+  Definition init: t := fun _ => Cell.init.
+
+  Variant message_to: forall (msg:Message.t) (loc:Loc.t) (to:Time.t), Prop :=
+  | message_to_intro
+      val released loc to
+      (TS: Time.le ((View.rlx (View.unwrap released)) loc) to):
+    message_to (Message.mk val released) loc to
+  .
+  #[global] Hint Constructors message_to: core.
+
+  Definition closed_timemap (times:TimeMap.t) (mem:t): Prop :=
+    forall loc, exists from val released,
+      get loc (times loc) mem = Some (from, Message.mk val released).
+
+  Variant closed_view (view:View.t) (mem:t): Prop :=
+  | closed_view_intro
+      (PLN: closed_timemap (View.pln view) mem)
+      (RLX: closed_timemap (View.rlx view) mem)
+  .
+  #[global] Hint Constructors closed_view: core.
+
+  Variant closed_opt_view: forall (view:option View.t) (mem:t), Prop :=
+  | closed_opt_view_some
+      view mem
+      (CLOSED: closed_view view mem):
+      closed_opt_view (Some view) mem
+  | closed_opt_view_none
+      mem:
+      closed_opt_view None mem
+  .
+  #[global] Hint Constructors closed_opt_view: core.
+
+  Variant closed_message: forall (msg:Message.t) (mem:t), Prop :=
+  | closed_message_intro
+      val released mem
+      (CLOSED: closed_opt_view released mem):
+    closed_message (Message.mk val released) mem
+  .
+  #[global] Hint Constructors closed_message: core.
+
+
+  Definition inhabited (mem:t): Prop :=
+    forall loc, get loc Time.bot mem = Some (Time.bot, Message.elt).
+  #[global] Hint Unfold inhabited: core.
+
+  Variant closed (mem:t): Prop :=
+  | closed_intro
+      (CLOSED: forall loc from to msg
+                 (MSG: get loc to mem = Some (from, msg)),
+          <<MSG_WF: Message.wf msg>> /\
+          <<MSG_TS: message_to msg loc to>> /\
+          <<MSG_CLOSED: closed_message msg mem>>)
+      (INHABITED: inhabited mem)
+  .
+  #[global] Hint Constructors closed: core.
+
+  Lemma closed_timemap_bot
+        mem
+        (INHABITED: inhabited mem):
+    closed_timemap TimeMap.bot mem.
+  Proof. ii. esplits. eapply INHABITED. Qed.
+
+  Lemma closed_view_bot
+        mem
+        (INHABITED: inhabited mem):
+    closed_view View.bot mem.
+  Proof. econs; apply closed_timemap_bot; auto. Qed.
+
+  Lemma unwrap_closed_opt_view
+        view mem
+        (CLOSED: closed_opt_view view mem)
+        (INHABITED: inhabited mem):
+    closed_view (View.unwrap view) mem.
+  Proof.
+    inv CLOSED; ss. apply closed_view_bot. ss.
+  Qed.
+
+  Lemma le_closed_timemap
+        tm mem1 mem2
+        (LE: le mem1 mem2)
+        (CLOSED: Memory.closed_timemap tm mem1):
+    Memory.closed_timemap tm mem2.
+  Proof.
+    ii. exploit CLOSED; eauto. i. des.
+    esplits; eauto.
+  Qed.
+
+  Lemma le_closed_view
+        view mem1 mem2
+        (LE: le mem1 mem2)
+        (CLOSED: Memory.closed_view view mem1):
+    Memory.closed_view view mem2.
+  Proof.
+    inv CLOSED. econs; eauto using le_closed_timemap.
+  Qed.
+
+  Lemma le_closed_opt_view
+        view mem1 mem2
+        (LE: le mem1 mem2)
+        (CLOSED: Memory.closed_opt_view view mem1):
+    Memory.closed_opt_view view mem2.
+  Proof.
+    inv CLOSED; econs.
+    eapply le_closed_view; eauto.
+  Qed.
+
+  Lemma le_closed_message
+        msg mem1 mem2
+        (LE: le mem1 mem2)
+        (CLOSED: Memory.closed_message msg mem1):
+    Memory.closed_message msg mem2.
+  Proof.
+    inv CLOSED; econs.
+    eapply le_closed_opt_view; eauto.
+  Qed.
+
+  Lemma init_closed: closed init.
+  Proof.
+    econs; i; ss.
+    unfold get, init, Cell.get, Cell.init in MSG. ss.
+    apply DOMap.singleton_find_inv in MSG. des. inv MSG0.
+    splits; ss. econs. refl.
+  Qed.
+
+  Variant add (mem1:t) (loc:Loc.t) (from to:Time.t) (msg:Message.t) (mem2:t): Prop :=
+  | add_intro
+      r
+      (ADD: Cell.add (mem1 loc) from to msg r)
+      (MEM2: mem2 = LocFun.add loc r mem1)
+  .
+  #[global] Hint Constructors add: core.
+
+  Variant future_imm (mem1 mem2:t): Prop :=
+  | future_imm_intro
+      loc from to msg
+      (ADD: add mem1 loc from to msg mem2)
+      (CLOSED: closed_message msg mem2)
+      (TS: message_to msg loc to)
+  .
+  #[global] Hint Constructors future_imm: core.
+
+  Definition future := rtc future_imm.
+  #[global] Hint Unfold future: core.
+
+
+  (* Lemmas on add & future *)
+
+  Lemma add_ts
+        mem1 mem2 loc from to msg
+        (ADD: add mem1 loc from to msg mem2):
+    Time.lt from to.
+  Proof.
+    inv ADD. inv ADD0. ss.
+  Qed.
+
+  Lemma add_o
+        mem2 mem1 loc from to msg
+        l t
+        (ADD: add mem1 loc from to msg mem2):
+    get l t mem2 =
+    if loc_ts_eq_dec (l, t) (loc, to)
+    then Some (from, msg)
+    else get l t mem1.
+  Proof.
+    inv ADD. unfold get, LocFun.add. condtac.
+    - subst. erewrite Cell.add_o; eauto.
+      repeat (condtac; subst; des; ss; try congr).
+    - repeat (condtac; subst; des; ss; try congr).
+  Qed.
+
+  Lemma add_get0
+        mem1 loc from1 to1 msg1 mem2
+        (ADD: add mem1 loc from1 to1 msg1 mem2):
+    <<GET: get loc to1 mem1 = None>> /\
+    <<GET: get loc to1 mem2 = Some (from1, msg1)>>.
+  Proof.
+    inv ADD. eapply Cell.add_get0; eauto.
+    unfold get, Cell.get, LocFun.add. condtac; ss.
+  Qed.
+
+  Lemma add_get1
+        m1 loc from to msg m2
+        l f t m
+        (ADD: add m1 loc from to msg m2)
+        (GET1: get l t m1 = Some (f, m)):
+    get l t m2 = Some (f, m).
+  Proof.
+    erewrite add_o; eauto. condtac; ss.
+    des. subst. exploit add_get0; eauto. i. des. congr.
+  Qed.
+
+  Lemma add_get_diff
+        mem1 loc from to msg mem2
+        loc'
+        (ADD: add mem1 loc from to msg mem2)
+        (LOC: loc' <> loc):
+    forall to', get loc' to' mem2 = get loc' to' mem1.
+  Proof.
+    i. erewrite add_o; eauto. condtac; ss. des. ss.
+  Qed.
+
+  Lemma future_get1
+        loc from to msg mem1 mem2
+        (FUTURE: future mem1 mem2)
+        (GET: get loc to mem1 = Some (from, msg)):
+    <<GET: get loc to mem2 = Some (from, msg)>>.
+  Proof.
+    revert from msg GET.
+    induction FUTURE; eauto. i.
+    inv H. eauto using add_get1.
+  Qed.
+
+
+  (* inhabited *)
+
+  Lemma add_inhabited
+        mem1 mem2 loc from to msg
+        (ADD: add mem1 loc from to msg mem2)
+        (INHABITED: inhabited mem1):
+    <<INHABITED: inhabited mem2>>.
+  Proof.
+    ii. erewrite add_o; eauto. condtac; ss.
+    des. subst. inv ADD. inv ADD0. inv TO.
+  Qed.
+
+  Lemma future_inhabited
+        mem1 mem2
+        (FUTURE: future mem1 mem2)
+        (INHABITED: inhabited mem1):
+    inhabited mem2.
+  Proof.
+    revert INHABITED.
+    induction FUTURE; eauto. i. inv H.
+    apply IHFUTURE.
+    eapply add_inhabited; eauto.
+  Qed.
+
+
+  (* le *)
+
+  Lemma add_le
+        mem1 loc from to msg mem2
+        (ADD: add mem1 loc from to msg mem2):
+    le mem1 mem2.
+  Proof.
+    ii. eapply Memory.add_get1; eauto.
+  Qed.
+
+  Lemma future_le
+        mem1 mem2
+        (FUTURE: future mem1 mem2):
+    le mem1 mem2.
+  Proof.
+    induction FUTURE; try refl.
+    etrans; eauto.
+    inv H. eapply add_le; eauto.
+  Qed.
+
+
+  (* Lemmas on closedness *)
+
+  Lemma join_closed_timemap
+        lhs rhs mem
+        (LHS: closed_timemap lhs mem)
+        (RHS: closed_timemap rhs mem):
+    closed_timemap (TimeMap.join lhs rhs) mem.
+  Proof.
+    ii. unfold TimeMap.join.
+    destruct (Time.join_cases (lhs loc) (rhs loc)) as [X|X]; rewrite X.
+    - apply LHS.
+    - apply RHS.
+  Qed.
+
+  Lemma join_closed_view
+        lhs rhs mem
+        (LHS: closed_view lhs mem)
+        (RHS: closed_view rhs mem):
+    closed_view (View.join lhs rhs) mem.
+  Proof.
+    econs.
+    - apply join_closed_timemap.
+      + apply LHS.
+      + apply RHS.
+    - apply join_closed_timemap.
+      + apply LHS.
+      + apply RHS.
+  Qed.
+
+  Lemma add_closed_timemap
+        times
+        mem1 loc from to msg mem2
+        (ADD: add mem1 loc from to msg mem2)
+        (CLOSED: closed_timemap times mem1):
+    closed_timemap times mem2.
+  Proof.
+    ii. erewrite add_o; eauto. condtac; ss.
+    des. subst. exfalso.
+    specialize (CLOSED loc). des.
+    exploit add_get0; eauto. i. des. congr.
+  Qed.
+
+  Lemma add_closed_view
+        view
+        mem1 loc from to msg mem2
+        (ADD: add mem1 loc from to msg mem2)
+        (CLOSED: closed_view view mem1):
+    closed_view view mem2.
+  Proof.
+    inv CLOSED. econs; eauto.
+    - eapply add_closed_timemap; eauto.
+    - eapply add_closed_timemap; eauto.
+  Qed.
+
+  Lemma add_closed_opt_view
+        view
+        mem1 loc from to msg mem2
+        (ADD: add mem1 loc from to msg mem2)
+        (CLOSED: closed_opt_view view mem1):
+    closed_opt_view view mem2.
+  Proof.
+    inv CLOSED; econs. eapply add_closed_view; eauto.
+  Qed.
+
+  Lemma add_closed_message
+        msg'
+        mem1 loc from to msg mem2
+        (ADD: add mem1 loc from to msg mem2)
+        (CLOSED: closed_message msg' mem1):
+    closed_message msg' mem2.
+  Proof.
+    destruct msg'; ss. inv CLOSED. econs.
+    eapply add_closed_opt_view; eauto.
+  Qed.
+
+  Lemma add_closed
+        mem1 loc from to msg mem2
+        (ADD: add mem1 loc from to msg mem2)
+        (CLOSED: closed mem1)
+        (MSG_CLOSED: closed_message msg mem2)
+        (MSG_TS: message_to msg loc to):
+    closed mem2.
+  Proof.
+    inv CLOSED. econs.
+    - i. revert MSG. erewrite add_o; eauto. condtac; ss.
+      + des. subst. i. inv MSG. splits; auto.
+        inv ADD. inv ADD0. auto.
+      + guardH o. i. exploit CLOSED0; eauto. i. des. splits; auto.
+        eapply add_closed_message; eauto.
+    - eapply add_inhabited; eauto.
+  Qed.
+
+  Lemma future_closed_timemap
+        times mem1 mem2
+        (CLOSED: closed_timemap times mem1)
+        (FUTURE: future mem1 mem2):
+    closed_timemap times mem2.
+  Proof.
+    revert CLOSED. induction FUTURE; auto. i.
+    apply IHFUTURE. inv H.
+    eapply add_closed_timemap; eauto.
+  Qed.
+
+  Lemma future_closed_view
+        view mem1 mem2
+        (FUTURE: future mem1 mem2)
+        (CLOSED: closed_view view mem1):
+    closed_view view mem2.
+  Proof.
+    revert CLOSED. induction FUTURE; auto. i.
+    apply IHFUTURE. inv H.
+    eapply add_closed_view; eauto.
+  Qed.
+
+  Lemma future_closed_opt_view
+        view mem1 mem2
+        (FUTURE: future mem1 mem2)
+        (CLOSED: closed_opt_view view mem1):
+    closed_opt_view view mem2.
+  Proof.
+    inv CLOSED; econs. eapply future_closed_view; eauto.
+  Qed.
+
+  Lemma future_closed_message
+        msg mem1 mem2
+        (FUTURE: future mem1 mem2)
+        (CLOSED: closed_message msg mem1):
+    closed_message msg mem2.
+  Proof.
+    inv CLOSED; econs. eapply future_closed_opt_view; eauto.
+  Qed.
+
+  Lemma future_closed
+        mem1 mem2
+        (FUTURE: future mem1 mem2)
+        (CLOSED: closed mem1):
+    closed mem2.
+  Proof.
+    revert CLOSED. induction FUTURE; auto. i.
+    apply IHFUTURE. inv H.
+    eapply add_closed; eauto.
+  Qed.
+
+  Lemma singleton_closed_timemap
+        loc from to val released mem
+        (GET: get loc to mem = Some (from, Message.mk val released))
+        (INHABITED: inhabited mem):
+    closed_timemap (TimeMap.singleton loc to) mem.
+  Proof.
+    unfold TimeMap.singleton, LocFun.add, LocFun.find. ii. condtac.
+    - subst. eauto.
+    - apply closed_timemap_bot. auto.
+  Qed.
+
+  Lemma singleton_ur_closed_view
+        loc from to val released mem
+        (GET: get loc to mem = Some (from, Message.mk val released))
+        (INHABITED: inhabited mem):
+    closed_view (View.singleton_ur loc to) mem.
+  Proof.
+    econs; s.
+    - eapply singleton_closed_timemap; eauto.
+    - eapply singleton_closed_timemap; eauto.
+  Qed.
+
+  Lemma singleton_rw_closed_view
+        loc from to val released mem
+        (GET: get loc to mem = Some (from, Message.mk val released))
+        (INHABITED: inhabited mem):
+    closed_view (View.singleton_rw loc to) mem.
+  Proof.
+    econs; s.
+    - apply closed_timemap_bot. auto.
+    - eapply singleton_closed_timemap; eauto.
+  Qed.
+
+  Lemma singleton_ur_if_closed_view
+        cond loc from to val released mem
+        (GET: get loc to mem = Some (from, Message.mk val released))
+        (INHABITED: inhabited mem):
+    closed_view (View.singleton_ur_if cond loc to) mem.
+  Proof.
+    destruct cond; ss.
+    - eapply singleton_ur_closed_view; eauto.
+    - eapply singleton_rw_closed_view; eauto.
+  Qed.
+
+
+  (* future *)
+
+  Lemma add_future
+        mem1 loc from to msg mem2
+        (ADD: add mem1 loc from to msg mem2)
+        (CLOSED1: closed mem1)
+        (MSG_CLOSED: closed_message msg mem2)
+        (MSG_TS: message_to msg loc to):
+    <<CLOSED2: closed mem2>> /\
+    <<FUTURE: future mem1 mem2>> /\
+    <<MSG_WF: Message.wf msg>>.
+  Proof.
+    hexploit add_inhabited; try apply CLOSED1; eauto. i. splits.
+    - eapply add_closed; eauto.
+    - econs 2; eauto.
+    - inv ADD. inv ADD0. ss.
+  Qed.
+
+
+  (* Lemmas on max_timemap *)
+
+  Definition max_ts (loc:Loc.t) (mem:t): Time.t :=
+    Cell.max_ts (mem loc).
+
+  Lemma max_ts_spec
+        loc ts from msg mem
+        (GET: get loc ts mem = Some (from, msg)):
+    <<GET: exists from msg, get loc (max_ts loc mem) mem = Some (from, msg)>> /\
+    <<MAX: Time.le ts (max_ts loc mem)>>.
+  Proof. eapply Cell.max_ts_spec; eauto. Qed.
+
+  Lemma max_ts_spec2
+        tm mem loc
+        (CLOSED: closed_timemap tm mem):
+    Time.le (tm loc) (max_ts loc mem).
+  Proof.
+    exploit CLOSED. i. des.
+    eapply max_ts_spec. eauto.
+  Qed.
+
+  Definition max_timemap (mem:t): TimeMap.t :=
+    fun loc => max_ts loc mem.
+
+  Lemma max_timemap_spec
+        tm mem
+        (TIMEMAP: closed_timemap tm mem)
+        (INHABITED: inhabited mem):
+    TimeMap.le tm (max_timemap mem).
+  Proof.
+    ii. specialize (INHABITED loc). des.
+    exploit TIMEMAP. i. des.
+    eapply max_ts_spec; eauto.
+  Qed.
+
+  Definition max_view (mem:t): View.t :=
+    View.mk (max_timemap mem) (max_timemap mem).
+
+  Lemma max_view_wf mem: View.wf (max_view mem).
+  Proof. econs. refl. Qed.
+
+  Lemma max_view_spec tm mem
+        (VIEW: closed_view tm mem)
+        (INHABITED: inhabited mem):
+    View.le tm (max_view mem).
+  Proof.
+    econs; apply max_timemap_spec; try apply VIEW; auto.
+  Qed.
+
+  Lemma closed_timemap_add
+        loc from to val released mem tm
+        (GET: get loc to mem = Some (from, Message.mk val released))
+        (CLOSED: closed_timemap tm mem):
+    closed_timemap (TimeMap.add loc to tm) mem.
+  Proof.
+    ii. unfold TimeMap.add. condtac.
+    - subst. esplits; eauto.
+    - apply CLOSED.
+  Qed.
+
+
+  (* Lemmas on existence of memory op *)
+
+  Lemma add_exists
+        mem1 loc from to msg
+        (DISJOINT: forall to2 from2 msg2
+                     (GET2: get loc to2 mem1 = Some (from2, msg2)),
+            Interval.disjoint (from, to) (from2, to2))
+        (TO1: Time.lt from to)
+        (MSG_WF: Message.wf msg):
+    exists mem2, add mem1 loc from to msg mem2.
+  Proof.
+    exploit Cell.add_exists; eauto. i. des.
+    eexists. econs; eauto.
+  Qed.
+
+  Lemma add_exists_max_ts
+        mem1 loc to msg
+        (TS: Time.lt (max_ts loc mem1) to)
+        (MSG_WF: Message.wf msg):
+    exists mem2,
+      add mem1 loc (max_ts loc mem1) to msg mem2.
+  Proof.
+    eapply add_exists; eauto.
+    i. exploit max_ts_spec; eauto. i. des.
+    ii. inv LHS. inv RHS. ss.
+    rewrite MAX in TO0. eapply Time.lt_strorder. eapply TimeFacts.le_lt_lt; eauto.
+  Qed.
+
+  Lemma add_exists_le
+        mem1' mem1 loc from to msg mem2
+        (LE: le mem1' mem1)
+        (ADD: add mem1 loc from to msg mem2):
+    exists mem2', add mem1' loc from to msg mem2'.
+  Proof.
+    inv ADD.
+    exploit Cell.add_exists_le; eauto.
+    { ii. eapply LE. eauto. }
+    i. des.
+    eexists. econs; eauto.
+  Qed.
+
+  Lemma add_inj
+        mem loc to from msg mem1 mem2
+        (REMOVE1: Memory.add mem loc from to msg mem1)
+        (REMOVE2: Memory.add mem loc from to msg mem2):
+    mem1 = mem2.
+  Proof.
+    apply Memory.ext. i.
+    setoid_rewrite Memory.add_o; eauto.
+  Qed.
+End Memory.
